Sad

Access.v
@@ -50,6 +50,27 @@ Inductive access (ad : addr) (m : mem) : tm -> Prop :=
                                access ad m <{acq t1 t2   }>
   .
 
+(* inversion --------------------------------------------------------------- *)
+
+Local Ltac _acc tt :=
+  match goal with
+  | H : access _ _ <{unit     }>   |- _ => inv H
+  | H : access _ _ <{nat _    }>   |- _ => inv H
+  | H : access _ _ <{var _    }>   |- _ => inv H
+  | H : access _ _ <{fn _ _ _ }>   |- _ => tt H
+  | H : access _ _ <{call _ _ }>   |- _ => tt H
+  | H : access _ _ <{& _ : _  }>   |- _ => tt H
+  | H : access _ _ <{new _ : _}>   |- _ => tt H
+  | H : access _ _ <{* _      }>   |- _ => tt H
+  | H : access _ _ <{_ := _   }>   |- _ => tt H
+  | H : access _ _ <{acq _  _ }>   |- _ => tt H
+  | H : access _ _ <{cr _ _   }>   |- _ => inv H
+  | H : access _ _ <{spawn _  }>   |- _ => inv H
+  end.
+
+Ltac inv_acc  := _acc inv.
+Ltac invc_acc := _acc invc.
+
 (* ------------------------------------------------------------------------- *)
 (* write-access                                                              *)
 (* ------------------------------------------------------------------------- *)
@@ -90,6 +111,27 @@ Inductive write_access (ad : addr) (m : mem) : tm  -> Prop :=
                                 write_access ad m <{acq t1 t2 }>
   .
 
+(* inversion --------------------------------------------------------------- *)
+
+Local Ltac _wacc tt :=
+  match goal with
+  | H : write_access _ _ <{unit     }>   |- _ => inv H
+  | H : write_access _ _ <{nat _    }>   |- _ => inv H
+  | H : write_access _ _ <{var _    }>   |- _ => inv H
+  | H : write_access _ _ <{fn _ _ _ }>   |- _ => tt H
+  | H : write_access _ _ <{call _ _ }>   |- _ => tt H
+  | H : write_access _ _ <{& _ : _  }>   |- _ => tt H
+  | H : write_access _ _ <{new _ : _}>   |- _ => tt H
+  | H : write_access _ _ <{* _      }>   |- _ => tt H
+  | H : write_access _ _ <{_ := _   }>   |- _ => tt H
+  | H : write_access _ _ <{acq _  _ }>   |- _ => tt H
+  | H : write_access _ _ <{cr _ _   }>   |- _ => inv H
+  | H : write_access _ _ <{spawn _  }>   |- _ => inv H
+  end.
+
+Ltac inv_wacc  := _wacc inv.
+Ltac invc_wacc := _wacc invc.
+
 (* ------------------------------------------------------------------------- *)
 (* read-access                                                              *)
 (* ------------------------------------------------------------------------- *)
@@ -98,110 +140,66 @@ Definition read_access (ad : addr) (m : mem) (t : tm) :=
   access ad m t /\ ~ write_access ad m t.
 
 (* ------------------------------------------------------------------------- *)
-(* guards                                                                    *)
+(* exclusive-access                                                          *)
 (* ------------------------------------------------------------------------- *)
 
-Definition guards adx ad m :=
-  exists T, m[adx].T = `x&T` /\ access ad m m[adx].t.
+(* Access exclusively through a critical region. *)
+Inductive exclusive_access (adx ad : addr) (m : mem) : tm -> Prop :=
+  | xacc_fun    : forall x Tx t, exclusive_access adx ad m t  ->
+                                 exclusive_access adx ad m <{fn x Tx t }>
 
-(* lemmas ------------------------------------------------------------------ *)
+  | xacc_call1  : forall t1 t2,  exclusive_access adx ad m t1 ->
+                                 exclusive_access adx ad m <{call t1 t2}>
 
-Lemma guards_adx_lt : forall adx ad m,
-  guards adx ad m ->
-  adx < #m.
-Proof.
-  intros * [? [? ?]].
-  decompose sum (lt_eq_lt_dec adx (#m)); subst; trivial; sigma; discriminate.
-Qed.
+  | xacc_call2  : forall t1 t2,  exclusive_access adx ad m t2 ->
+                                 exclusive_access adx ad m <{call t1 t2}>
 
-(* ------------------------------------------------------------------------- *)
-(* guarded-access                                                            *)
-(* ------------------------------------------------------------------------- *)
+  | xacc_new    : forall T t,    exclusive_access adx ad m t  ->
+                                 exclusive_access adx ad m <{new t : T }>
 
-(* Access (exclusively) through a critical region. *)
-Inductive guarded_access (adx ad : addr) (m : mem) : tm -> Prop :=
-  | xacc_fun    : forall x Tx t, guarded_access adx ad m t  ->
-                                 guarded_access adx ad m <{fn x Tx t }>
+  | xacc_load   : forall t,      exclusive_access adx ad m t  ->
+                                 exclusive_access adx ad m <{*t        }>
 
-  | xacc_call1  : forall t1 t2,  guarded_access adx ad m t1 ->
-                                 guarded_access adx ad m <{call t1 t2}>
+  | xacc_asg1   : forall t1 t2,  exclusive_access adx ad m t1 ->
+                                 exclusive_access adx ad m <{t1 := t2  }>
 
-  | xacc_call2  : forall t1 t2,  guarded_access adx ad m t2 ->
-                                 guarded_access adx ad m <{call t1 t2}>
+  | xacc_asg2   : forall t1 t2,  exclusive_access adx ad m t2 ->
+                                 exclusive_access adx ad m <{t1 := t2  }>
 
-  | xacc_new    : forall T t,    guarded_access adx ad m t  ->
-                                 guarded_access adx ad m <{new t : T }>
+  | xacc_acq1   : forall t1 t2,  exclusive_access adx ad m t1 ->
+                                 exclusive_access adx ad m <{acq t1 t2 }>
 
-  | xacc_load   : forall t,      guarded_access adx ad m t  ->
-                                 guarded_access adx ad m <{*t        }>
+  | xacc_acq2   : forall t1 t2,  exclusive_access adx ad m t2 ->
+                                 exclusive_access adx ad m <{acq t1 t2 }>
 
-  | xacc_asg1   : forall t1 t2,  guarded_access adx ad m t1 ->
-                                 guarded_access adx ad m <{t1 := t2  }>
+  | xacc_cr_eq  : forall t,      access ad m t                ->
+                                 exclusive_access adx ad m <{cr adx t  }>
 
-  | xacc_asg2   : forall t1 t2,  guarded_access adx ad m t2 ->
-                                 guarded_access adx ad m <{t1 := t2  }>
-
-  | xacc_acq1   : forall t1 t2,  guarded_access adx ad m t1 ->
-                                 guarded_access adx ad m <{acq t1 t2 }>
-
-  | xacc_acq2   : forall t1 t2,  guarded_access adx ad m t2 ->
-                                 guarded_access adx ad m <{acq t1 t2 }>
-
-  | xacc_cr_eq  : forall t,      access ad m t              ->
-                                 guarded_access adx ad m <{cr adx t  }>
-
-  | xacc_cr_neq : forall adx' t, adx <> adx'                ->
-                                 guarded_access adx ad m t  ->
-                                 guarded_access adx ad m <{cr adx' t }>
+  | xacc_cr_neq : forall adx' t, adx <> adx'                  ->
+                                 exclusive_access adx ad m t  ->
+                                 exclusive_access adx ad m <{cr adx' t }>
   .
 
-(* ------------------------------------------------------------------------- *)
-(* inversions                                                                *)
-(* ------------------------------------------------------------------------- *)
-
-Local Ltac _acc_racc_wacc P tt :=
-  match goal with
-  | H : P _ _ <{unit     }>   |- _ => inv H
-  | H : P _ _ <{nat _    }>   |- _ => inv H
-  | H : P _ _ <{var _    }>   |- _ => inv H
-  | H : P _ _ <{fn _ _ _ }>   |- _ => tt H
-  | H : P _ _ <{call _ _ }>   |- _ => tt H
-  | H : P _ _ <{& _ : _  }>   |- _ => tt H
-  | H : P _ _ <{new _ : _}>   |- _ => tt H
-  | H : P _ _ <{* _      }>   |- _ => tt H
-  | H : P _ _ <{_ := _   }>   |- _ => tt H
-  | H : P _ _ <{acq _  _ }>   |- _ => tt H
-  | H : P _ _ <{cr _ _   }>   |- _ => inv H
-  | H : P _ _ <{spawn _  }>   |- _ => inv H
-  end.
-
-Ltac inv_acc  := _acc_racc_wacc access inv.
-Ltac invc_acc := _acc_racc_wacc access invc.
-
-Ltac inv_wacc  := _acc_racc_wacc write_access inv.
-Ltac invc_wacc := _acc_racc_wacc write_access invc.
-
-Ltac inv_racc  := _acc_racc_wacc read_access inv.
-Ltac invc_racc := _acc_racc_wacc read_access invc.
+(* inversion --------------------------------------------------------------- *)
 
 Local Ltac _xacc tt :=
   match goal with
-  | H : guarded_access _ _ _ <{unit     }>   |- _ => inv H
-  | H : guarded_access _ _ _ <{nat _    }>   |- _ => inv H
-  | H : guarded_access _ _ _ <{var _    }>   |- _ => inv H
-  | H : guarded_access _ _ _ <{fn _ _ _ }>   |- _ => tt H
-  | H : guarded_access _ _ _ <{call _ _ }>   |- _ => tt H
-  | H : guarded_access _ _ _ <{& _ : _  }>   |- _ => inv H
-  | H : guarded_access _ _ _ <{new _ : _}>   |- _ => tt H
-  | H : guarded_access _ _ _ <{* _      }>   |- _ => tt H
-  | H : guarded_access _ _ _ <{_ := _   }>   |- _ => tt H
-  | H : guarded_access _ _ _ <{acq _  _ }>   |- _ => tt H
-  | H : guarded_access _ _ _ <{cr _ _   }>   |- _ => tt H
-  | H : guarded_access _ _ _ <{spawn _  }>   |- _ => inv H
+  | H : exclusive_access _ _ _ <{unit     }>   |- _ => inv H
+  | H : exclusive_access _ _ _ <{nat _    }>   |- _ => inv H
+  | H : exclusive_access _ _ _ <{var _    }>   |- _ => inv H
+  | H : exclusive_access _ _ _ <{fn _ _ _ }>   |- _ => tt H
+  | H : exclusive_access _ _ _ <{call _ _ }>   |- _ => tt H
+  | H : exclusive_access _ _ _ <{& _ : _  }>   |- _ => inv H
+  | H : exclusive_access _ _ _ <{new _ : _}>   |- _ => tt H
+  | H : exclusive_access _ _ _ <{* _      }>   |- _ => tt H
+  | H : exclusive_access _ _ _ <{_ := _   }>   |- _ => tt H
+  | H : exclusive_access _ _ _ <{acq _  _ }>   |- _ => tt H
+  | H : exclusive_access _ _ _ <{cr _ _   }>   |- _ => tt H
+  | H : exclusive_access _ _ _ <{spawn _  }>   |- _ => inv H
   end.
 
-Ltac inv_cacc  := _xacc inv.
-Ltac invc_cacc := _xacc invc.
+Ltac inv_xacc  := _xacc inv.
+Ltac invc_xacc := _xacc invc.
 
 (* ------------------------------------------------------------------------- *)
 (* not-access                                                                *)
@@ -259,14 +257,14 @@ Lemma nacc_spawn : forall ad m t,
 Proof. solve_cons_nacc. Qed.
 
 #[export] Hint Resolve
-  nacc_unit nacc_nat
-  nacc_var nacc_fun nacc_call
-  nacc_ref nacc_new nacc_load nacc_asg
-  nacc_acq nacc_cr
+  nacc_unit  nacc_nat
+  nacc_var   nacc_fun nacc_call
+  nacc_ref   nacc_new nacc_load nacc_asg
+  nacc_acq   nacc_cr
   nacc_spawn
   : not_access.
 
-(* inversions -------------------------------------------------------------- *)
+(* inversion --------------------------------------------------------------- *)
 
 Local Ltac solve_inv_nacc := 
   intros; try split; eauto using access.
@@ -328,6 +326,46 @@ Ltac invc_nacc :=
   | H : ~ access _ _ <{cr _ _     }> |- _ => clear H
   | H : ~ access _ _ <{spawn _    }> |- _ => clear H
   end.
+
+(* lemmas ------------------------------------------------------------------ *)
+
+Lemma nacc_mem : forall m t,
+  forall_memory m (valid_references m) ->
+  valid_references m t ->
+  (* --- *)
+  ~ access (#m) m t.
+Proof.
+  intros ** Hacc. induction Hacc; invc_vr; eauto.
+Qed.
+
+(* preservation lemmas ----------------------------------------------------- *)
+
+Local Lemma nacc_subst : forall ad m x tx t,
+  ~ access ad m t ->
+  ~ access ad m tx ->
+  ~ access ad m <{[x := tx] t}>.
+Proof.
+  intros * Ht Htx. induction t; trivial; simpl in *; invc_nacc;
+  try destruct str_eq_dec; eauto with not_access.
+Qed.
+
+Local Lemma nacc_mem_set1 : forall m t ad ad' t' T',
+  ~ access ad m t' ->
+  ~ access ad m t  ->
+  ~ access ad m[ad'.tT <- t' T'] t.
+Proof.
+  intros ** Hacc. induction Hacc; eauto using access;
+  repeat omicron; invc_nacc; eauto with not_access.
+Qed.
+
+Local Lemma nacc_mem_set2 : forall m t ad ad' c,
+  ~ access ad' m t ->
+  ~ access ad  m t ->
+  ~ access ad  m[ad' <- c] t.
+Proof.
+  intros ** Hacc.
+  induction Hacc; repeat invc_nacc; eauto using access; sigma; eauto.
+Qed.
 
 (* ------------------------------------------------------------------------- *)
 (* not-write-access                                                          *)
@@ -393,19 +431,35 @@ Ltac invc_nwacc :=
   | H : ~ write_access _ _ <{spawn _    }> |- _ => clear H
   end.
 
+(* ------------------------------------------------------------------------- *)
+(* basic lemmas                                                              *)
+(* ------------------------------------------------------------------------- *)
 
+Lemma wacc_then_acc : forall ad m t,
+  write_access ad m t ->
+  access ad m t.
+Proof.
+  intros * Hwacc. induction Hwacc; eauto using access.
+Qed.
 
+Lemma racc_then_acc : forall ad m t,
+  read_access ad m t ->
+  access ad m t.
+Proof.
+  intros * [? _]. assumption.
+Qed.
 
-
-
-
-
-
-
-
+Lemma safe_then_nwacc : forall m ad ad' T,
+  forall_memory m value ->
+  empty |-- m[ad'].t is `Safe T` ->
+  ~ write_access ad m m[ad'].t.
+Proof.
+  intros * Hval **. intros ?.
+  destruct (Hval ad'); invc_typeof; invc_wacc; eauto.
+Qed.
 
 (* ------------------------------------------------------------------------- *)
-(* ptyp preservation                                                         *)
+(* pointer types                                                             *)
 (* ------------------------------------------------------------------------- *)
 
 Theorem ptyp_preservation : forall m1 m2 ths1 ths2 tid e ad,
@@ -419,36 +473,6 @@ Proof.
   omicron; trivial. ind_tstep; repeat invc_vr; eauto.
 Qed.
 
-(* ------------------------------------------------------------------------- *)
-(* ptyp & wacc/racc                                                          *)
-(* ------------------------------------------------------------------------- *)
-
-Lemma wacc_then_acc : forall ad m t,
-  write_access ad m t ->
-  access ad m t.
-Proof.
-  intros * Hwacc. induction Hwacc; eauto using access.
-Qed.
-
-Corollary racc_then_acc : forall ad m t,
-  read_access ad m t ->
-  access ad m t.
-Proof.
-  intros * [? _]. assumption.
-Qed.
-
-Lemma nwacc_from_safe_type : forall m ad ad' T,
-  forall_memory m value ->
-  empty |-- m[ad'].t is `Safe T` ->
-  ~ write_access ad m m[ad'].t.
-Proof.
-  intros * Hval **. intros ?.
-  specialize (Hval ad'); simpl in *.
-  destruct Hval; inv_typeof; inv_wacc; eauto.
-Qed.
-
-(* ------------------------------------------------------------------------- *)
-
 Lemma ptyp_wacc_correlation : forall m t ad,
   forall_memory m value ->
   forall_memory m (valid_references m) ->
@@ -458,9 +482,9 @@ Lemma ptyp_wacc_correlation : forall m t ad,
   write_access ad m t <-> (exists T, m[ad].T = `w&T`).
 Proof.
   intros * ? Hmvr ? Hacc. split.
-  - intros Hwacc. clear Hacc. induction Hwacc; inv_vr; eauto.
-  - intros [? Heq]. induction Hacc; inv_vr; eauto using write_access.
-    exfalso. eapply nwacc_from_safe_type; eauto.
+  - intros Hwacc. clear Hacc. induction Hwacc; invc_vr; eauto.
+  - intros [? ?]. induction Hacc; invc_vr; eauto using write_access.
+    exfalso. eapply safe_then_nwacc; eauto.
 Qed.
 
 Corollary wacc_by_association : forall m t t' ad,
@@ -487,7 +511,7 @@ Lemma ptyp_racc_correlation : forall m t ad,
   read_access ad m t <-> (exists T, m[ad].T = `r&T`).
 Proof.
   intros * Hval ? ? Hacc. split; intros [? ?].
-  - induction Hacc; invc_vr; invc_nwacc; eauto using nwacc_from_safe_type.
+  - induction Hacc; invc_vr; invc_nwacc; eauto using safe_then_nwacc.
   - split; trivial. induction Hacc; intros ?; invc_vr; inv_wacc; eauto;
     eapply IHHacc; eauto using wacc_by_association.
 Qed.
@@ -504,7 +528,7 @@ Corollary racc_by_association : forall m t t' ad,
 Proof.
   intros * ? ? ? ? ? Hracc.
   eapply ptyp_racc_correlation; eauto.
-  specialize Hracc as Hracc'. destruct Hracc' as [? ?].
+  duplicate Hracc Hracc'. destruct Hracc' as [? ?].
   eapply ptyp_racc_correlation; eauto.
 Qed.
 
@@ -522,80 +546,200 @@ Theorem ptyp_racc_wacc_contradiction : forall m1 m2 t1 t2 ad,
   False.
 Proof.
   intros until 7. intros Hracc Hwacc.
-  eapply ptyp_racc_correlation in Hracc as [? Htyp1]; eauto using racc_then_acc.
-  eapply ptyp_wacc_correlation in Hwacc as [? Htyp2]; eauto using wacc_then_acc.
+  eapply ptyp_racc_correlation in Hracc as [? Htyp1];
+  eauto using racc_then_acc.
+  eapply ptyp_wacc_correlation in Hwacc as [? Htyp2];
+  eauto using wacc_then_acc.
   rewrite Htyp1 in *. rewrite Htyp2 in *. discriminate.
 Qed.
 
-
-
-
-
-
-
-
-
-
-
-
-
-
-
-
-
-
-
-
-
 (* ------------------------------------------------------------------------- *)
-(* valid_access_types                                                        *)
+(* access-promise-1                                                          *)
 (* ------------------------------------------------------------------------- *)
 
-Definition valid_access_types (m : mem) := forall ad1 ad2 T1 T2,
-  access ad1 m m[ad2].t ->
-  m[ad1].T = `w&T1` ->
-  m[ad2].T = `r&T2` ->
+Definition access_promise1 (ad : addr) (m : mem) (t : tm) :=  forall adx T,
+  m[ad].T = `w&T` ->
+  exclusive_access adx ad m t ->
+  access ad m t ->
   False.
+
+(* constructors ------------------------------------------------------------ *)
+
+Local Lemma ap1_unit : forall ad m,
+  access_promise1 ad m <{unit}>.
+Proof.
+  intros until 3. invc_xacc.
+Qed.
+
+Local Lemma ap1_nat : forall ad m n,
+  access_promise1 ad m <{nat n}>.
+Proof.
+  intros until 3. invc_xacc.
+Qed.
+
+Local Lemma ap1_ref : forall ad m n,
+  access_promise1 ad m <{nat n}>.
+Proof.
+  intros until 3. invc_xacc.
+Qed.
+
+Local Lemma ap1_var : forall ad m x,
+  access_promise1 ad m <{var x}>.
+Proof.
+  intros until 3. invc_xacc.
+Qed.
+
+Local Lemma ap1_fun : forall ad m x Tx t,
+  access_promise1 ad m t -> access_promise1 ad m <{fn x Tx t}>.
+Proof.
+  intros until 4. invc_acc; invc_xacc. eauto.
+Qed.
+
+Local Lemma ap1_call : forall ad m t1 t2,
+  access_promise1 ad m t1 ->
+  access_promise1 ad m t2 ->
+  access_promise1 ad m <{call t1 t2}>.
+Proof.
+  intros. intros until 3. invc_acc; invc_xacc; eauto.
+Abort.
+
+#[export] Hint Resolve
+  ap1_unit  ap1_nat
+  ap1_var   ap1_fun
+  ap1_ref
+  : ap1.
+
+(* inversion --------------------------------------------------------------- *)
+
+Local Ltac solve_inv_ap1 :=
+  intros; try split; intros until 3; eauto using access, exclusive_access. 
+
+Local Lemma inv_ap1_fun : forall ad m x Tx t,
+  access_promise1 ad m <{fn x Tx t}> ->
+  access_promise1 ad m t.
+Proof. solve_inv_ap1. Qed.
+
+Local Lemma inv_ap1_call : forall ad m t1 t2,
+  access_promise1 ad m <{call t1 t2}> ->
+  access_promise1 ad m t1 /\ access_promise1 ad m t2.
+Proof. solve_inv_ap1. Qed.
+
+Ltac dup_apply1 H L := specialize H as H'; eapply L in H.
+Ltac dup_apply2 H L := specialize H as H'; eapply L in H as [? ?].
+
+Ltac inv_ap1 :=
+  match goal with
+  | H : access_promise1 _ _ <{fn _ _ _   }> |- _ => dup_apply1 H inv_ap1_fun
+  | H : access_promise1 _ _ <{call _ _   }> |- _ => dup_apply2 H inv_ap1_call
+  end.
 
 (* preservation ------------------------------------------------------------ *)
 
-Local Lemma acc_mem_setX : forall m t ad ad' X,
-  forall_memory m (valid_references m) ->
-  valid_references m t ->
-  (* --- *)
-  access ad m t ->
-  access ad m[ad'.X <- X] t.
+Local Lemma acc_subst_backwards : forall ad m x tx t,
+  access ad m <{[x := tx] t}> ->
+  access ad m tx \/ access ad m t.
 Proof.
-  intros * ? ? Hacc. induction Hacc; repeat invc_vr; eauto using access.
-  - eapply acc_memR; trivial. omicron; eauto.
-  - eapply acc_memW; trivial. omicron; eauto.
+  intros. induction t; eauto; simpl in *; try destruct str_eq_dec; eauto;
+  invc_acc; aspecialize;
+  match goal with H : _ \/ _ |- _ => destruct H end;
+  eauto using access.
 Qed.
 
-Local Lemma acc_mem_setX' : forall m t ad ad' X,
-  ad' < #m ->
-  access ad m[ad'.X <- X] t ->
-  access ad m t.
+Local Lemma xacc_subst_backwads : forall adx ad m x tx t,
+  exclusive_access adx ad m <{ [x := tx] t }> ->
+  (exclusive_access adx ad m tx \/
+   exclusive_access adx ad m t  \/
+   access ad m <{[x := tx] t}>  ).
 Proof.
-  intros * ? Hacc.
-  induction Hacc; repeat invc_vr; eauto using access.
-  - eapply acc_memR; trivial. omicron; eauto.
-  - eapply acc_memW; trivial. omicron; eauto.
-Qed.
-
-Local Lemma vat_preservation_mstep : forall m1 m2 t1 t2 e,
-  valid_access_types m1 ->
-  m1 / t1 ==[e]==> m2 / t2 ->
-  valid_access_types m2.
-Proof.
-  intros. invc_mstep; trivial.
-  - admit.
-  - ind_tstep; eauto; repeat clean.
-    intros ad1 ad2 T1 T2 Hacc Had1 Had2. repeat omicron; subst;
-    try discriminate.
-    + admit.
-    + admit.
-    + admit.
+  intros. induction t; eauto; simpl in *; try destruct str_eq_dec; eauto;
+  inv_xacc; try aspecialize;
+  try solve [
+    match goal with H : _ \/ _ \/ _ |- _ => decompose sum H end;
+    eauto using access, exclusive_access
+  ].
+  - eapply acc_subst_backwards in H1 as [? | ?];
+    eauto using exclusive_access.
+    exfalso.
+    admit.
+  - destruct IHt as [? | [? | ?]]; eauto.
+    + right. left. eapply xacc_cr_neq; eauto.
+    + exfalso. (*H0 e H3*)
 Abort.
+
+Local Lemma ap1_subst : forall ad m x tx Tx t,
+  access_promise1 ad m <{call (fn x Tx t) tx}> ->
+  access_promise1 ad m t ->
+  access_promise1 ad m tx ->
+  access_promise1 ad m <{[x := tx] t}>.
+Proof.
+  intros * H Ht Htx. intros until 3.
+  specialize (Ht adx T H0).
+  specialize (Htx adx T H0).
+  assert (Hacc : access ad m tx \/ access ad m t)
+    by eauto using acc_subst_backwards.
+  destruct Hacc; repeat aspecialize;
+  eauto using access, exclusive_access.
+  - admit.
+  - admit.
+Abort.
+
+Local Lemma ap1_preservation_none : forall ad m t1 t2,
+  access_promise1 ad m t1 ->
+  t1 --[e_none]--> t2 ->
+  access_promise1 ad m t2.
+Proof.
+  intros * Hap ?. ind_tstep; repeat clean.
+  - inv_ap1. repeat aspecialize. intros until 3.
+    invc_xacc; invc_acc; eauto.
+    + assert (exclusive_access adx ad m t1) by admit.
+      eauto using access, exclusive_access.
+    + assert (access ad m t1) by admit.
+      eauto using access, exclusive_access.
+  - admit.
+  - inv_ap1. eapply inv_ap1_fun in H0 as ?.
+
+
+
+
+    intros until 3; eauto using access, exclusive_access.
+  - intros until 2.
+Qed.
+
+Local Lemma ap1_preservation_mstep : forall m1 m2 ths tid t e,
+  xacc_acc_promise m1 ths ->
+  m1 / ths[tid] ==[e]==> m2 / t ->
+  xacc_acc_promise m2 ths[tid <- t].
+Proof.
+  intros. invc_mstep.
+  - admit.
+  - admit.
+  - admit.
+  - admit.
+  - admit.
+  - admit.
+Qed.
+
+
+
+
+
+
+
+
+
+
+
+
+
+
+
+
+(* ------------------------------------------------------------------------- *)
+(* guards                                                                    *)
+(* ------------------------------------------------------------------------- *)
+
+Definition guards adx ad m :=
+  exists T, m[adx].T = `x&T` /\ access ad m m[adx].t.
 
 (* ------------------------------------------------------------------------- *)
 (* guard-promise                                                             *)
@@ -605,6 +749,63 @@ Definition guard_promise (m : mem) (t : tm) := forall adx ad T,
   m[ad].T = `w&T` ->
   guards adx ad m ->
   ~ access ad m t.
+
+Local Ltac solve_cons_gp :=
+  intros ** ? ? ? ? ?; eauto with not_access.
+
+Lemma gp_unit : forall m,
+  guard_promise m <{unit}>.
+Proof. solve_cons_gp. Qed.
+
+Lemma gp_nat : forall m n,
+  guard_promise m <{nat n}>.
+Proof. solve_cons_gp. Qed.
+
+Lemma gp_var : forall m x,
+  guard_promise m <{var x}>.
+Proof. solve_cons_gp. Qed.
+
+Lemma gp_fun : forall m x Tx t,
+  guard_promise m t -> guard_promise m <{fn x Tx t}>.
+Proof. solve_cons_gp. Qed.
+
+Lemma gp_call : forall m t1 t2,
+  guard_promise m t1 -> guard_promise m t2 -> guard_promise m <{call t1 t2}>.
+Proof. solve_cons_gp. Qed.
+
+(* gp_ref *)
+
+Lemma gp_new : forall m t T,
+  guard_promise m t -> guard_promise m <{new t : T}>.
+Proof. solve_cons_gp. Qed.
+
+Lemma gp_load : forall m t,
+  guard_promise m t -> guard_promise m <{*t}>.
+Proof. solve_cons_gp. Qed.
+
+Lemma gp_asg : forall m t1 t2,
+  guard_promise m t1 -> guard_promise m t2 -> guard_promise m <{t1 := t2}>.
+Proof. solve_cons_gp. Qed.
+
+Lemma gp_acq : forall m t1 t2,
+  guard_promise m t1 -> guard_promise m t2 -> guard_promise m <{acq t1 t2}>.
+Proof. solve_cons_gp. Qed.
+
+Lemma gp_cr : forall m adx t,
+  guard_promise m <{cr adx t}>.
+Proof. solve_cons_gp. Qed.
+
+Lemma gp_spawn : forall m t,
+  guard_promise m <{spawn t}>.
+Proof. solve_cons_gp. Qed.
+
+#[export] Hint Resolve
+  gp_unit gp_nat
+  gp_var  gp_fun gp_call
+  gp_new  gp_load gp_asg
+  gp_acq  gp_cr
+  gp_spawn
+  : guard_promise.
 
 (* inversion --------------------------------------------------------------- *)
 
@@ -652,16 +853,90 @@ Ltac invc_gp :=
   | H : guard_promise _ <{spawn _  }> |- _ => clear H
   end.
 
-(* preservation ------------------------------------------------------------ *)
+(* lemmas ------------------------------------------------------------------ *)
 
-Local Lemma nacc_subst : forall ad m x tx t,
-  ~ access ad m t ->
-  ~ access ad m tx ->
-  ~ access ad m <{[x := tx] t}>.
+Lemma gp_tstep_write_term : forall m t1 t2 ad t T,
+  guard_promise m t1 ->
+  t1 --[e_write ad t T]--> t2 ->
+  guard_promise m t.
 Proof.
-  intros * Ht Htx. induction t; trivial; simpl in *; invc_nacc;
-  try destruct str_eq_dec; eauto with not_access.
+  intros. ind_tstep; try solve [invc_gp; eauto with guard_promise].
+  repeat clean.
+Abort.
+
+(* preservation lemmas ----------------------------------------------------- *)
+
+Local Lemma acc_mem_set_X_backwards : forall m t ad ad' X,
+  forall_memory m (valid_references m) ->
+  valid_references m t ->
+  (* --- *)
+  access ad m[ad'.X <- X] t ->
+  access ad m t.
+Proof.
+  intros * ? ? Hacc. induction Hacc; invc_vr; eauto using access;
+  omicron; eauto using access.
 Qed.
+
+Local Lemma acc_mem_set_tT_backwards1 : forall m t ad ad' t' T',
+  ~ access ad m t' ->
+  (* --- *)
+  access ad m[ad'.tT <- t' T'] t ->
+  access ad m t.
+Proof.
+  intros * ? Hacc. remember (m[ad'.tT <- t' T']) as m'.
+  induction Hacc; inv Heqm'; eauto using access;
+  match goal with |- access _ _ <{& ?ad : _}> => rename ad into ad'' end;
+  destruct (nat_eq_dec ad' ad''); subst; try (sigma; eauto using access);
+  destruct (nat_eq_dec ad'' ad); subst; eauto using access;
+  rewrite (set_get_eq cell_default) in IHHacc; try contradiction;
+  omicron; eauto; inv_acc.
+Qed.
+
+Lemma acc_mem_set_tT_backwards2 : forall m t ad ad' c,
+  ~ access ad' m t ->
+  (* --- *)
+  access ad m[ad' <- c] t ->
+  access ad m t.
+Proof.
+  intros * ? Hacc. induction Hacc; invc_nacc; eauto using access;
+  sigma; eauto using access.
+Qed.
+
+Local Lemma gp_mem_set_X : forall m t ad X,
+  forall_memory m (valid_references m) ->
+  valid_references m t ->
+  (* --- *)
+  guard_promise m t ->
+  guard_promise m[ad.X <- X] t.
+Proof.
+  intros * ? ? Hgp. induction t;
+  try solve [try inv_vr; invc_gp; eauto with guard_promise].
+  intros ? ? ? ? [? [? ?]] ?.
+  repeat omicron; eauto; try discriminate;
+  eapply Hgp; eauto; try eexists; eauto using acc_mem_set_X_backwards.
+Qed.
+
+Local Lemma gp_mem_set_tT : forall m t ad t' T',
+  forall_memory m (valid_references m) ->
+  valid_references m t ->
+  (* --- *)
+  m[ad].T = `w&T'` ->
+  guard_promise m t ->
+  guard_promise m[ad.tT <- t' `w&T'`] t.
+Proof.
+  intros * ? ? ? Hgp. induction t;
+  try solve [try inv_vr; invc_gp; eauto with guard_promise].
+  intros ? ? ? ? [? [? ?]] ?.
+  repeat omicron; eauto; try discriminate.
+  - invc H2.
+    eapply Hgp; eauto.
+    + eexists. admit.
+    + eapply acc_mem_set_tT_backwards1; eauto.
+      admit.
+  - admit.
+Abort.
+
+(* preservation ------------------------------------------------------------ *)
 
 Local Lemma gp_preservation_none : forall m t1 t2,
   guard_promise m t1 ->
@@ -672,6 +947,11 @@ Proof.
   unfold guard_promise in *; eauto using nacc_subst with not_access.
 Qed.
 
+
+
+
+
+
 Lemma nacc_mem_add : forall m t ad tT,
   ~ access (#m) m t ->
   (* --- *)
@@ -681,46 +961,100 @@ Proof.
   intros ** Hacc. induction Hacc; repeat invc_nacc; eauto; omicron; eauto.
 Qed.
 
-Local Lemma gp_mem_add : forall m t t' T',
+Local Lemma acc_mem_add : forall ad m t t' T',
+  ad < #m ->
+  access ad m t ->
+  access ad (m +++ (t', T', false)) t.
+Proof.
+  intros * ? Hacc. induction Hacc; eauto using access;
+  (eapply acc_memR || eapply acc_memW); eauto; omicron; eauto; invc_acc.
+Qed.
+
+Lemma acc_mem_add_backwards : forall m t ad c,
+  forall_memory m (valid_references m) ->
   valid_references m t ->
   (* --- *)
-  guard_promise m t ->
-  guard_promise (m +++ (t', T', false)) t.
+  access ad (m +++ c) t ->
+  access ad m t.
 Proof.
-  intros. induction t; repeat invc_vr; invc_gp; 
-  try solve [repeat aspecialize;
-             unfold guard_promise; intros; eauto with not_access].
-  - rename a into ad'.
-    intros adx ad T'' Had Hguards.
-    specialize (H0 adx ad T'').
-    omicron.
-    + aspecialize.
-    eapply nacc_mem_add; eauto.
-    unfold guard_promise; intros; eauto with not_access.
+  intros * ? Hvr Hacc.
+  assert (Hnacc : ~ access (#m) m t) by eauto using nacc_vr_length.
+  clear Hvr. induction Hacc; invc_nacc; eauto using access;
+  omicron; eauto using access; invc_acc.
+Qed.
+
+Local Lemma guards_mem_add : forall adx ad m t T,
+  ad < #m ->
+  guards adx ad m ->
+  guards adx ad (m +++ (t, T, false)).
+Proof.
+  intros * ? [Tx [Hadx Hacc]]. exists Tx. split;
+  omicron; eauto using acc_mem_add; discriminate.
+Qed.
+
+Local Lemma guards_mem_add_backwards : forall adx ad m t T,
+  forall_memory m (valid_references m) ->
+  (* --- *)
+  adx < #m ->
+  guards adx ad (m +++ (t, T, false)) ->
+  guards adx ad m.
+Proof.
+  intros * ? ? [Tx [Hadx Hacc]]. sigma. eexists.
+  eauto using acc_mem_add_backwards.
 Qed.
 
 Local Lemma gp_preservation_alloc : forall m t1 t2 t T,
+  forall_memory m (valid_references m) ->
+  valid_references m t1 ->
+  (* --- *)
   guard_promise m t1 ->
   t1 --[e_alloc (#m) t T]--> t2 ->
   guard_promise (m +++ (t, T, false)) t2.
 Proof.
-  intros. ind_tstep; invc_gp;
+  intros. ind_tstep; invc_vr; invc_gp;
   repeat clean.
-  - repeat aspecialize. 
-    intros adx ad Tx Had Hguards Hacc. omicron.
-    +
-  
+  - repeat aspecialize.
+    intros adx ad Tw Had Hguards.
+    eapply nacc_call; eauto.
+    destruct Hguards as [Tx [Hadx Hacc]]. omicron; subst.
+    + omicron; subst; try discriminate.
+      * eapply acc_mem_add_backwards in Hacc; eauto.
+        specialize (H1 adx ad Tw Had).
+        eapply nacc_mem_add; eauto using nacc_vr_length.
+        eapply H1.
+        eexists; eauto.
+      * eapply acc_mem_add_backwards in Hacc; eauto.
+        contradict Hacc.
+        eapply nacc_vr_length; eauto.
+    + omicron; try discriminate.
+      eapply acc_mem_add_backwards in Hacc; eauto using vr_tstep_alloc_term.
+      eapply nacc_mem_add; eauto using nacc_vr_length.
+      admit.
+    + invc_acc.
+Abort.
+
+
+x& (Nat)
+
+x& (&w (w& Nat))
+
+m.acq (&t
+---
+
+
+m.set (t)
+
+
+new t : x&T --[e]--> new t' : x&T
+
+new t : ... --[e_none]--> newx ad t
+
+new v : x&T --[e]--> &ad : x&T
 
 
 
-  - unfold guard_promise in *; eauto with not_access.
 
 
-  intros. ind_tstep; intros until 2; repeat invc_gp;
-  unfold guard_promise in *; eauto with not_access. eapply nacc_ref.
-  - intros ?. subst. sigma. discriminate.
-  - sigma. eauto with not_access.
-Qed.
 
 Local Lemma gp_preservation_read : forall m t1 t2 ad,
   well_typed_term t1 ->
@@ -742,22 +1076,38 @@ Proof.
   repeat invc_typeof; invc_nacc; trivial. 
 Qed.
 
-Local Lemma gp_preservation_write : forall m t1 t2 ad t T,
-  guard_promise m t1 ->
+Local Lemma wtt_tstep_write_type : forall t1 t2 ad t T,
+  well_typed_term t1 ->
   t1 --[e_write ad t T]--> t2 ->
-  guard_promise m t2.
+  exists Tw, T = `w&Tw`.
 Proof.
-  intros. ind_tstep; intros until 2; repeat invc_gp;
-  unfold guard_promise in *; eauto with not_access.
+  intros * [T ?] **. gendep T. ind_tstep; intros; repeat invc_typeof; eauto.
 Qed.
 
+Local Lemma gp_preservation_write : forall m t1 t2 ad t T,
+  well_typed_term t1 ->
+  (* --- *)
+  guard_promise m t1 ->
+  t1 --[e_write ad t T]--> t2 ->
+  guard_promise m[ad.tT <- t T] t2.
+Proof.
+  intros. ind_tstep; invc_wtt; invc_gp.
+  - eapply gp_call; eauto.
+    duplicate H1 Htstep.
+    eapply wtt_tstep_write_type in H1 as [? ?]; eauto; subst.
+    clean.
+Abort.
+
 Local Lemma gp_preservation_acq : forall m t1 t2 ad t,
+  forall_memory m (valid_references m) ->
+  valid_references m t1 ->
+  (* --- *)
   guard_promise m t1 ->
   t1 --[e_acq ad t]--> t2 ->
-  guard_promise m t2.
+  guard_promise m[ad.X <- true] t2.
 Proof.
-  intros. ind_tstep; intros until 2; repeat invc_gp;
-  unfold guard_promise in *; eauto with not_access.
+  intros. ind_tstep; invc_vr; invc_gp;
+  eauto using gp_mem_set_X with guard_promise.
 Qed.
 
 Local Lemma gp_preservation_rel : forall m t1 t2 ad,
@@ -768,11 +1118,11 @@ Local Lemma gp_preservation_rel : forall m t1 t2 ad,
   (* --- *)
   guard_promise m t1 ->
   t1 --[e_rel ad]--> t2 ->
-  guard_promise m t2.
+  guard_promise m[ad.X <- false] t2.
 Proof.
-  intros.
-  ind_tstep; intros until 2; invc_vr; invc_sb; invc_gp;
-  try solve [unfold guard_promise in *; eauto with not_access].
+  intros. ind_tstep; invc_vr; invc_sb; invc_gp;
+  eauto using gp_mem_set_X with guard_promise.
+  eapply gp_mem_set_X; eauto. intros until 2.
   invc_sval; eauto with not_access; invc_vr; intros ?; invc_acc; eauto.
   eapply nwacc_from_safe_type; eauto.
   eapply ptyp_wacc_correlation; eauto.
@@ -788,8 +1138,11 @@ Proof.
 Qed.
 
 Local Lemma gp_preservation_mstep : forall m1 m2 t1 t2 e,
+  forall_memory m1 value ->
   well_typed_term t1 ->
+  forall_memory m1 (valid_references m1) ->
   valid_references m1 t1 ->
+  safe_boundaries t1 ->
   (* --- *)
   guard_promise m1 t1 ->
   m1 / t1 ==[e]==> m2 / t2 ->
@@ -797,12 +1150,14 @@ Local Lemma gp_preservation_mstep : forall m1 m2 t1 t2 e,
 Proof.
   intros. invc_mstep;
   eauto using gp_preservation_none;
-  eauto using gp_preservation_alloc;
+  (* eauto using gp_preservation_alloc; *)
   eauto using gp_preservation_read;
-  eauto using gp_preservation_write;
+  (* eauto using gp_preservation_write; *)
   eauto using gp_preservation_acq;
   eauto using gp_preservation_rel;
   eauto using gp_preservation_spawn.
+  - admit.
+  - admit.
 Qed.
 
 Theorem gp_preservation : forall m1 m2 ths1 ths2 tid e,
@@ -813,14 +1168,7 @@ Theorem gp_preservation : forall m1 m2 ths1 ths2 tid e,
   m1 / ths1 ~~[tid, e]~~> m2 / ths2 ->
   forall_threads ths2 (guard_promise m2).
 Proof.
-  intros. invc_cstep; try invc_mstep; intros ?; omicron; eauto;
-  eauto using gp_preservation_none;
-  eauto using gp_preservation_alloc;
-  eauto using gp_preservation_read;
-  eauto using gp_preservation_write;
-  eauto using gp_preservation_acq;
-  eauto using gp_preservation_rel;
-  eauto using gp_preservation_spawn.
+  intros. invc_cstep.
 Qed.
 
 
