Boundaries.v
@@ -85,3 +85,6 @@ Local Ltac _sb tt :=
 Ltac inv_sb  := _sb inv.
 Ltac invc_sb := _sb invc.
 
+(* preservation ------------------------------------------------------------ *)
+
+(* TODO *)
